crnf.v
@@ -1,0 +1,153 @@
+Require Export weak.
+Require Import cases.
+
+Lemma lem_wh_step_1 : forall t w u s, step_wh t w -> step_wh t u -> inf_wh u s ->
+                                      exists x, step_wh_eq s x /\ inf_wh w x.
+Proof.
+  intros t w u s H1 H2 H3.
+  exists s.
+  assert (HH: w == u) by eauto using lem_step_wh_unique.
+  rewrite HH; clear HH.
+  pose_term_eq; ycrush.
+Qed.
+
+Lemma lem_wh_step_commute : forall t t1 t2, inf_wh t t1 -> step_wh t t2 ->
+                                            exists t3, step_wh_eq t1 t3 /\ inf_wh t2 t3.
+Proof.
+  intros t t1 t2 H1 H2.
+  revert t1 H1.
+  induction H2; subst.
+  - intros t1 H2.
+    assert (step_wh x y) by ycrush.
+    inversion_clear H; subst.
+    inversion_clear H2; subst.
+    + generalize (lem_red_wh_rev x _ H); sintuition.
+      * eapply lem_wh_step_1; pose_inf_wh; ycrush.
+      * rewrite H4 in *; exfalso; yelles 1.
+    + generalize (lem_red_wh_rev x _ H); sintuition.
+      * eapply lem_wh_step_1; pose_inf_wh; ycrush.
+      * rewrite H4 in *; exfalso; yelles 1.
+    + generalize (lem_red_wh_rev x _ H); sintuition.
+      * eapply lem_wh_step_1; pose_inf_wh; ycrush.
+      * rewrite H6 in *.
+        inversion_clear H1; subst; sintuition; fold term_eq inf_wh in *.
+        rewrite H2 in *; rewrite H7 in *.
+        inversion_clear H4; subst; sintuition; fold term_eq inf_wh in *;
+          try solve [ pose lem_red_wh_from_abs; yforwarding; yelles 1 ].
+        assert (HH: x1 == t0) by (pose lem_red_wh_from_abs; ycrush).
+        rewrite HH in *; clear HH.
+        exists (x'0 [0 := y']).
+        split.
+        ** pose lem_step_wh_redex; ycrush.
+        ** pose lem_inf_wh_subst; ycrush.
+    + generalize (lem_red_wh_rev x _ H); sintuition.
+      * eapply lem_wh_step_1; pose_inf_wh; ycrush.
+      * rewrite H5 in *; exfalso; yelles 1.
+  - intros t1 H1.
+    rewrite H in *.
+    assert (step_wh (app x y) (app x' y')) by (pose_term_eq; ycrush).
+    inversion_clear H1; subst.
+    + generalize (lem_red_wh_rev (app x y') _ H3); sintuition.
+      * eapply lem_wh_step_1; rewrite H in *; pose_inf_wh; ycrush.
+      * exfalso; yelles 1.
+    + generalize (lem_red_wh_rev (app x y') _ H3); sintuition.
+      * eapply lem_wh_step_1; rewrite H in *; pose_inf_wh; ycrush.
+      * exfalso; yelles 1.
+    + generalize (lem_red_wh_rev (app x y') _ H3); sintuition.
+      * eapply lem_wh_step_1; rewrite H in *; pose_inf_wh; ycrush.
+      * inversion_clear H6; subst; sintuition; fold term_eq inf_wh in *.
+        rewrite <- H1 in *; rewrite <- H7 in *.
+        generalize (IHstep_wh x'0 H4); sintuition.
+        exists (app t3 y'0).
+        split.
+        ** destruct H6; [ left | right ]; pose_term_eq; ycrush.
+        ** pose_inf_wh; ycrush.
+    + generalize (lem_red_wh_rev (app x y') _ H3); sintuition.
+      * eapply lem_wh_step_1; rewrite H in *; pose_inf_wh; ycrush.
+      * exfalso; yelles 1.
+Qed.
+
+Lemma lem_wh_commute : forall t t1 t2, inf_wh t t1 -> red_wh t t2 ->
+                                       exists t3, red_wh t1 t3 /\ inf_wh t2 t3.
+Proof.
+  intros t t1 t2 H1 H.
+  revert t1 H1.
+  destruct H as [n H]; induction H.
+  - intros; rewrite H in *; pose_red_wh; ycrush.
+  - intros t1 H1.
+    generalize (lem_wh_step_commute x t1 y H1 H); sintuition.
+    unfold step_wh_eq in *; pose_red_wh; ycrush.
+Qed.
+
+Lemma lem_rnf_red_wh : forall t s, inf_beta t s -> is_rnf s ->
+                                   exists s', is_rnf s' /\ red_wh t s' /\ inf_wh s' s.
+Proof.
+  intros t s H1 H2.
+  assert (H1w: inf_wh t s) by reasy (lem_inf_beta_to_inf_wh) Reconstr.Empty.
+  unfold is_rnf in H2.
+  destruct s.
+  - yelles 1.
+  - unfold is_rnf; exists (var n); pose_inf_wh; scrush.
+  - inversion_clear H1w; subst; fold inf_wh in *.
+    enough (is_rnf (app x y)) by (pose_inf_wh; scrush).
+    unfold is_rnf, is_abs, not; intros z HH ?; destruct z; yisolve.
+    assert (HH1: exists u, inf_wh x (abs u)) by reasy (lem_inf_beta_to_inf_wh) Reconstr.Empty.
+    assert (HH2: exists u, red_wh x (abs u)) by (clear -HH1; scrush).
+    clear HH1.
+    destruct HH2 as [u].
+    assert (HH3: exists r, inf_wh (abs u) r /\ red_wh s1 r) by
+        (clear -H5 H0; pose lem_wh_commute; ycrush).
+    destruct HH3 as [r [HH1 HH2]].
+    assert (is_abs r) by (clear -HH1; pose lem_inf_wh_from_abs; ycrush).
+    pose_inf_wh; pose lem_inf_wh_to_inf_beta; ycrush.
+  - inversion H1w; unfold is_rnf; exists (abs x); pose_inf_wh; scrush.
+Qed.
+
+Definition is_crnf t r := is_rnf r /\ forall s, inf_beta t s -> is_rnf s -> red_wh t r /\ inf_wh r s.
+Hint Unfold is_crnf.
+
+Add Parametric Morphism : is_rnf with
+    signature term_eq ==> iff as step_wh_mor.
+Proof.
+  split; unfold is_rnf; sauto; inversion H; ycrush.
+Qed.
+
+Lemma lem_crnf_exists : forall t, has_rnf t -> exists r, is_crnf t r.
+Proof.
+  intros t H.
+  unfold has_rnf in H.
+  destruct H as [t' [H1 H2]].
+  generalize (lem_rnf_red_wh t t' H2 H1); intro HH; destruct HH as [s [HH1 [HH2 HH3]]].
+  clear H2; revert HH1.
+  destruct HH2 as [n H].
+  induction H; intros.
+  - exists x; unfold is_crnf; split; intros; rewrite H in *; pose_red_wh; pose lem_inf_beta_to_inf_wh; ycrush.
+  - generalize (is_rnf_dec x); intro Hd; destruct Hd as [ Hd | Hd ].
+    + exists x; unfold is_crnf; pose_red_wh; pose lem_inf_beta_to_inf_wh; ycrush.
+    + unfold is_crnf in *.
+      generalize (IHstar_n HH3 HH1); intro HH; destruct HH as [r [Hr1 Hr2]].
+      exists r; split; eauto; intros.
+      generalize (lem_rnf_red_wh x s H2 H3); intro HH; destruct HH as [s' [H4 [H5 H6]]].
+      destruct H5 as [m H5].
+      inversion_clear H5; subst.
+      * exfalso; rewrite H7 in *; ycrush.
+      * assert (Hy0: y0 == y) by reasy (@weak.lem_step_wh_unique) Reconstr.Empty.
+        rewrite Hy0 in *; clear Hy0.
+        assert (red_wh y s') by ycrush.
+        assert (inf_beta y s) by (pose_inf_wh; pose lem_inf_wh_to_inf_beta; ycrush).
+        pose_red_wh; ycrush.
+Qed.
+
+Definition crnf0 t (p : has_rnf t) : { r | is_crnf t r }.
+  apply constructive_indefinite_description.
+  apply lem_crnf_exists.
+  assumption.
+Defined.
+
+Definition crnf t (p : has_rnf t) := proj1_sig (crnf0 t p).
+
+Lemma lem_crnf_is_crnf : forall t (p : has_rnf t), is_crnf t (crnf t p).
+Proof.
+  intros; unfold crnf.
+  destruct (crnf0 t p); sauto.
+Qed.
